lib/Benchmarks/SmallFilterProof.v
@@ -25,6 +25,70 @@ RegisterEnvCtors
   (BigBits.Suf, FirstOrderConfRelSimplified.Bits 1).
 *)
 
+Lemma drop_antecedent:
+  forall P Q: Prop, P -> (P -> Q) <-> Q.
+Proof.
+  tauto.
+Qed.
+
+Ltac crunch_foterm_ctx :=
+  match goal with
+  | H: context[interp_fm ?v ?g] |- _ =>
+      let temp := fresh "temp" in
+      set (temp := g) in H; vm_compute in temp; subst temp;
+      (let temp := fresh "temp1" in
+       set (temp := v) in H; vm_compute in temp; subst temp)
+  end.
+
+Ltac compile_fm H :=
+  erewrite simplify_entailment_correct
+    with (equiv0:=RelationClasses.eq_equivalence)
+         (St_eq_dec:=@Sum.St_eq_dec _ _ _ _ _ _)
+    in H;
+  rewrite compile_simplified_entailment_correct in H;
+  rewrite FirstOrderConfRelSimplified.simplify_concat_zero_fm_corr in H;
+  erewrite FirstOrderConfRelSimplified.simplify_eq_zero_fm_corr in H;
+  erewrite CompileFirstOrderConfRelSimplified.compile_simplified_fm_bv_correct in H;
+  crunch_foterm_ctx;
+  try rewrite !drop_antecedent with (P := state_template_sane _) in H
+      by apply P4A.P4A.cap';
+  try rewrite !drop_antecedent with (P := state_template_sane _) in H
+      by (unfold state_template_sane;
+          simpl;
+          autorewrite with size';
+          cbv;
+          autorewrite with op_fmapH; Lia.lia);
+  rewrite !drop_antecedent with (P := top' _ _ _ _ _ _ _ _) in H
+      by repeat match goal with
+                | |- ?x = ?x \/ _ => exact (or_introl eq_refl)
+                | |- ?x = ?y \/ _ => apply or_intror
+                | |- _ => cbn
+                end.
+
+Ltac remember_iff name hyp term :=
+  set (name := term);
+  assert (hyp: name <-> term) by reflexivity;
+  clearbody name.
+
+Ltac decide_entailment H P HP P_orig e :=
+  let Horig := fresh "Horig" in
+  set (P_orig := e);
+  remember_iff P HP e;
+  assert (Horig: P_orig <-> P)
+    by (rewrite HP; reflexivity);
+  compile_fm HP;
+  match goal with
+  | HP: P <-> interp_fm ?v ?f |- _ =>
+      time "smt check neg" check_interp_neg (interp_fm v f);
+      idtac "UNSAT";
+      assert (~ P_orig) by (rewrite -> Horig; rewrite -> HP; apply dummy_pf_false)
+  | HP: P <-> interp_fm ?v ?f |- _ =>
+      time "smt check pos" check_interp_pos (interp_fm v f);
+      idtac "SAT";
+      assert (P_orig) by (rewrite -> Horig; rewrite -> HP; apply dummy_pf_true)
+  | |- _ => idtac "undecided goal :("
+  end;
+  clear Horig.
 
 Lemma prebisim_incremental_sep:
   lang_equiv_state
@@ -79,7 +143,50 @@ Proof.
   }
   vm_compute Reachability.reachable_states.
   vm_compute mk_init.
-  time "build phase" repeat (time "single step" run_bisim).
-  time "close phase" close_bisim.
-  (* TODO Now how to handle the pre-bisimulation goal...? *)
-Admitted.
+  repeat match goal with
+         | |- pre_bisimulation ?a ?r_states ?wp ?R (?C :: _) _ _ =>
+             let H := fresh "H" in
+             let P := fresh "P" in
+             let HP := fresh "HP" in
+             let P_orig := fresh "P_orig" in
+             decide_entailment H P HP P_orig (interp_entailment a
+                                                                (fun q1 q2 =>
+                                                                   top' _ _ _ _ _ r_states
+                                                                        (conf_to_state_template q1)
+                                                                        (conf_to_state_template q2))
+                                                                ({| e_prem := R; e_concl := C |}));
+             match goal with
+             | HN: ~ P_orig |- _ =>
+                 time "extending" (extend_bisim' HN; clear HN)
+             | H: P_orig |- pre_bisimulation _ _ _ _ (?C :: _) _ _ =>
+                 time "skipping" (skip_bisim' H; clear H; try clear C)
+             end;
+             clear P HP P_orig
+         end.
+  match goal with
+  | |- pre_bisimulation _ ?r_states _ _ _ _ _ =>
+        apply PreBisimulationClose;
+         match goal with
+         | H:interp_conf_rel' ?C ?q1 ?q2
+           |- interp_crel _ _ ?P ?q1 ?q2 =>
+               let H0 := fresh "H0" in
+               assert
+                (H0 :
+                 interp_entailment'
+                   (fun q1 q2 =>
+                    top' _ _ _ _ _ r_states (conf_to_state_template q1)
+                      (conf_to_state_template q2)) {| e_prem := P; e_concl := C |}) by
+                (eapply simplify_entailment_correct';
+                  eapply compile_simplified_entailment_correct'; simpl; 
+                  intros; eapply FirstOrderConfRelSimplified.simplify_eq_zero_fm_corr;
+                  eapply compile_simplified_fm_bv_correct; crunch_foterm;
+                  match goal with
+                  | |- ?X => time "smt check pos" check_interp_pos X; apply dummy_pf_true
+                  end); apply H0; auto; unfold top', conf_to_state_template; 
+                destruct q1, q2; vm_compute in H;
+                repeat match goal with
+                       | H:_ /\ _ |- _ => idtac H; destruct H
+                       end; subst; simpl; tauto
+         end
+  end.
+Qed.
